FoC/Computability/Compiler/Core/EncodedRewriters/ClosedConfigRunner/Projection/Quoter/SourceRestFinishCore.lean
@@ -1,1 +1,1 @@
-import FoC.Computability.Compiler.Core.EncodedRewriters.ClosedConfigRunner.Projection.Quoter.SourceRestFinishCore.Construction
+import FoC.Computability.Compiler.Core.EncodedRewriters.ClosedConfigRunner.Projection.Quoter.SourceRestFinishCore.Final
